proof-libs/fstar/rust_primitives/Rust_primitives.BitVectors.fst
@@ -42,25 +42,20 @@ let mask_inv_opt_in_range #t (mask: int_t t {Some? (mask_inv_opt (v mask))})
 
 let get_bit_pow2_minus_one_i32 x nth
   = let n = Some?.v (mask_inv_opt x) in
-    mk_int_equiv_lemma #i32_inttype x;
     get_bit_pow2_minus_one #i32_inttype n nth
 
 let get_bit_pow2_minus_one_i16 x nth
   = let n = Some?.v (mask_inv_opt x) in
-    mk_int_equiv_lemma #i16_inttype x;
     get_bit_pow2_minus_one #i16_inttype n nth
 
 let get_bit_pow2_minus_one_u32 x nth
   = let n = Some?.v (mask_inv_opt x) in
-    mk_int_equiv_lemma #u32_inttype x;
     get_bit_pow2_minus_one #u32_inttype n nth
 
 let get_bit_pow2_minus_one_u16 x nth
   = let n = Some?.v (mask_inv_opt x) in
-    mk_int_equiv_lemma #u16_inttype x;
     get_bit_pow2_minus_one #u16_inttype n nth
 
 let get_bit_pow2_minus_one_u8 t x nth
   = let n = Some?.v (mask_inv_opt x) in
-    mk_int_equiv_lemma #u8_inttype x;
     get_bit_pow2_minus_one #u8_inttype n nth
